Smallstep Done
Signed-off-by: Satyender Yadav <satyenderyadav4993@gmail.com>

Smallstep.v
@@ -344,3 +344,758 @@ Proof.
 
 Module Temp5.
 
+Reserved Notation " t '=>' t' " (at level 40).
+
+Inductive step : tm -> tm -> Prop :=
+  | ST_IfTrue : forall t1 t2,
+      tif ttrue t1 t2 => t1
+  | ST_IfFalse : forall t1 t2,
+      tif tfalse t1 t2 => t2
+  | ST_If : forall t1 t1' t2 t3,
+      t1 => t1' ->
+      tif t1 t2 t3 => tif t1' t2 t3
+  | ST_Short : forall t1 t2,
+      value t2 ->
+      tif t1 t2 t2 => t2
+
+  where " t '=>' t' " := (step t t').
+
+Definition bool_step_prop4 :=
+         tif
+            (tif ttrue ttrue ttrue)
+            tfalse
+            tfalse
+     =>
+         tfalse.
+
+Example bool_step_prop4_holds :
+  bool_step_prop4.
+Proof.
+  constructor. constructor.
+  Qed.
+
+Lemma negb_step_deterministic:
+  ~ deterministic step.
+Proof.
+  intros H. unfold deterministic in H.
+  assert(tif ttrue tfalse ttrue => tfalse).
+    constructor.
+  assert(tfalse = tif tfalse tfalse tfalse).
+  apply H with (tif (tif ttrue tfalse ttrue) tfalse tfalse);
+    constructor; constructor.
+  inversion H1. Qed.
+
+Theorem strong_progress : forall t,
+  value t \/ (exists t', t => t').
+Proof.
+  induction t.
+    apply or_introl; constructor.
+    apply or_introl; constructor.
+    apply or_intror; inversion IHt1;
+      inversion H; subst.
+        exists t2; constructor.
+        exists t3; constructor.
+      exists (tif x t2 t3); constructor.
+      assumption.
+  Qed.
+
+Module Temp6.
+
+Reserved Notation " t '=>' t' " (at level 40).
+
+Inductive step : tm -> tm -> Prop :=
+  | ST_IfTrue : forall t1 t2,
+      tif ttrue t1 t2 => t1
+  | ST_IfFalse : forall t1 t2,
+      tif tfalse t1 t2 => t2
+  | ST_Short : forall t1 t2,
+      value t2 ->
+      tif t1 t2 t2 => t2
+
+  where " t '=>' t' " := (step t t').
+
+Theorem strong_progress : exists t,
+  ~ value t /\ ~(exists t', t => t').
+Proof.
+  exists (tif (tif tfalse tfalse ttrue) tfalse ttrue).
+  split; intros H; inversion H. inversion H0; subst.
+  inversion H4.
+  Qed.
+
+End Temp6.
+
+End Temp5.
+End Temp4.
+
+Inductive multi {X:Type} (R: relation X) : relation X :=
+  | multi_refl : forall (x : X), multi R x x
+  | multi_step : forall (x y z : X),
+                    R x y ->
+                    multi R y z ->
+                    multi R x z.
+
+Tactic Notation "multi_cases" tactic(first) ident(c) :=
+  first;
+  [ Case_aux c "multi_refl" | Case_aux c "multi_step" ].
+
+Definition multistep := multi step.
+Notation " t '=>*' t' " := (multistep t t') (at level 40).
+
+Theorem multi_R : forall (X:Type) (R:relation X) (x y : X),
+       R x y -> (multi R) x y.
+Proof.
+  intros X R x y H.
+  apply multi_step with y. apply H. apply multi_refl. Qed.
+
+Theorem multi_trans :
+  forall (X:Type) (R: relation X) (x y z : X),
+      multi R x y ->
+      multi R y z ->
+      multi R x z.
+Proof.
+  intros.
+  generalize dependent z.
+  induction H. intros; assumption.
+  intros. econstructor. apply H.
+  apply IHmulti. assumption.
+  Qed.
+
+Lemma test_multistep_1:
+      P
+        (P (C 0) (C 3))
+        (P (C 2) (C 4))
+   =>*
+      C ((0 + 3) + (2 + 4)).
+Proof.
+  econstructor. constructor. constructor.
+  econstructor. apply ST_Plus2; constructor.
+  econstructor. constructor. constructor.
+  Qed.
+
+Lemma test_multistep_2:
+  C 3 =>* C 3.
+Proof.
+  constructor. Qed.
+
+Lemma test_multistep_3:
+      P (C 0) (C 3)
+   =>*
+      P (C 0) (C 3).
+Proof.
+  constructor. Qed.
+
+Lemma test_multistep_4:
+      P
+        (C 0)
+        (P
+          (C 2)
+          (P (C 0) (C 3)))
+  =>*
+      P
+        (C 0)
+        (C (2 + (0 + 3))).
+Proof.
+  econstructor. apply ST_Plus2. constructor.
+  apply ST_Plus2. constructor. constructor.
+  econstructor. apply ST_Plus2. constructor.
+  constructor. econstructor.
+  Qed.
+
+Definition step_normal_form := normal_form step.
+
+Definition normal_form_of (t t' : tm) :=
+  (t =>* t' /\ step_normal_form t').
+
+Theorem normal_forms_unique:
+  deterministic normal_form_of.
+Proof.
+  unfold deterministic. unfold normal_form_of. intros x y1 y2 P1 P2.
+  inversion P1 as [P11 P12]; clear P1. inversion P2 as [P21 P22]; clear P2.
+  generalize dependent y2.
+  induction P11.
+    destruct x; intros. inversion P21.
+      reflexivity.
+      inversion H.
+    assert(value (P x1 x2)).
+      apply nf_is_value; assumption.
+    inversion H.
+    intros. apply IHP11; try assumption.
+    inversion P21; subst. 
+      destruct y2.
+        inversion H.
+        assert (value (P y2_1 y2_2)).
+          apply nf_is_value; assumption.
+        inversion H0.
+        assert(y = y0).
+          eapply step_deterministic.
+          apply H. apply H0.
+        subst. apply H1.
+  Qed.
+
+Definition normalizing {X:Type} (R:relation X) :=
+  forall t, exists t',
+    (multi R) t t' /\ normal_form R t'.
+
+Lemma multistep_congr_1 : forall t1 t1' t2,
+     t1 =>* t1' ->
+     P t1 t2 =>* P t1' t2.
+Proof.
+  intros.
+  induction H. constructor.
+  econstructor. apply ST_Plus1. apply H.
+  assumption.
+  Qed.
+
+Lemma multistep_congr_2 : forall t1 t2 t2',
+     value t1 ->
+     t2 =>* t2' ->
+     P t1 t2 =>* P t1 t2'.
+Proof.
+  intros. induction H0.
+  constructor.
+  econstructor. apply ST_Plus2. assumption.
+  apply H0. assumption.
+  Qed.
+
+Theorem step_normalizing :
+  normalizing step.
+Proof.
+  unfold normalizing.
+  intros. induction t.
+    exists (C n).
+    split; try apply value_is_nf; try constructor.
+    inversion IHt1 as [t1' [H11 H12]].
+    inversion IHt2 as [t2' [H21 H22]].
+    assert(v1:value t1').
+      apply nf_is_value. assumption.
+    inversion v1.
+    assert(v2:value t2').
+      apply nf_is_value. assumption.
+    inversion v2.
+    exists(C (n + n0)). split.
+    assert(Hprime:P t1 t2 =>* P t1' t2').
+      eapply multi_trans.
+        apply multistep_congr_1. apply H11.
+        apply multistep_congr_2; assumption.
+    eapply multi_trans. apply Hprime.
+    subst. econstructor; constructor.
+    apply value_is_nf. constructor.
+  Qed.
+
+Theorem eval__multistep : forall t n,
+  t || n -> t =>* C n.
+Proof.
+  intros.
+  induction H. constructor.
+  eapply multi_trans.
+  assert(P t1 t2 =>* P (C n1) t2).
+    apply multistep_congr_1; assumption.
+    apply H1.
+  eapply multi_trans.
+    apply multistep_congr_2. constructor.
+    apply IHeval2.
+  econstructor; constructor.
+  Qed.
+
+Lemma step__eval : forall t t' n,
+     t => t' ->
+     t' || n ->
+     t || n.
+Proof.
+  intros t t' n Hs. generalize dependent n.
+  induction Hs; intros; inversion H; subst. constructor; constructor.
+  constructor. apply IHHs. assumption.
+  assumption. inversion H0; subst.
+  constructor. assumption. apply IHHs.
+  assumption.
+  Qed.
+
+Theorem multistep__eval : forall t t',
+  normal_form_of t t' -> exists n, t' = C n /\ t || n.
+Proof.
+  intros. unfold normal_form_of in H.
+  inversion H.
+  induction H0.
+  assert(value x).
+    apply nf_is_value. assumption.
+  inversion H0.
+  exists n. split; try reflexivity; try constructor.
+  assert(exists n : nat, z = C n /\ y || n).
+    apply IHmulti. split; assumption.
+    assumption.
+  inversion H3 as [n [H4 H5]]; clear H3.
+  exists n. split. assumption.
+  eapply step__eval. apply H0.
+  assumption.
+  Qed.
+
+Theorem evalF_eval : forall t n,
+  evalF t = n <-> t || n.
+Proof.
+  split; intros. generalize dependent n.
+  induction t; intros. simpl in H. subst. constructor.
+  simpl in H. rewrite <- H. constructor.
+    apply IHt1; reflexivity.
+    apply IHt2; reflexivity.
+  induction H.
+    reflexivity.
+    simpl. subst. reflexivity.
+  Qed.
+
+Module Combined.
+
+Inductive tm : Type :=
+  | C : nat -> tm
+  | P : tm -> tm -> tm
+  | ttrue : tm
+  | tfalse : tm
+  | tif : tm -> tm -> tm -> tm.
+
+Tactic Notation "tm_cases" tactic(first) ident(c) :=
+  first;
+  [ Case_aux c "C" | Case_aux c "P"
+  | Case_aux c "ttrue" | Case_aux c "tfalse" | Case_aux c "tif" ].
+
+Inductive value : tm -> Prop :=
+  | v_const : forall n, value (C n)
+  | v_true : value ttrue
+  | v_false : value tfalse.
+
+Reserved Notation " t '=>' t' " (at level 40).
+
+Inductive step : tm -> tm -> Prop :=
+  | ST_PlusConstConst : forall n1 n2,
+      P (C n1) (C n2) => C (n1 + n2)
+  | ST_Plus1 : forall t1 t1' t2,
+      t1 => t1' ->
+      P t1 t2 => P t1' t2
+  | ST_Plus2 : forall v1 t2 t2',
+      value v1 ->
+      t2 => t2' ->
+      P v1 t2 => P v1 t2'
+  | ST_IfTrue : forall t1 t2,
+      tif ttrue t1 t2 => t1
+  | ST_IfFalse : forall t1 t2,
+      tif tfalse t1 t2 => t2
+  | ST_If : forall t1 t1' t2 t3,
+      t1 => t1' ->
+      tif t1 t2 t3 => tif t1' t2 t3
+
+  where " t '=>' t' " := (step t t').
+
+Tactic Notation "step_cases" tactic(first) ident(c) :=
+  first;
+  [ Case_aux c "ST_PlusConstConst"
+  | Case_aux c "ST_Plus1" | Case_aux c "ST_Plus2"
+  | Case_aux c "ST_IfTrue" | Case_aux c "ST_IfFalse" | Case_aux c "ST_If" ].
+
+Theorem step_deterministic :
+  deterministic step.
+Proof.
+  intros x y z H. generalize dependent z.
+  induction H; intros.
+    inversion H; subst. reflexivity.
+    inversion H3.
+    inversion H4.
+    inversion H0; subst. inversion H.
+    replace t1'0 with t1'. reflexivity.
+    apply IHstep. assumption.
+    inversion H3; subst; inversion H.
+    inversion H1; subst. inversion H0.
+    inversion H; subst; inversion H5.
+    replace t2'0 with t2'. reflexivity.
+    apply IHstep. assumption.
+    inversion H; subst. reflexivity. inversion H4.
+    inversion H; subst. reflexivity. inversion H4.
+    inversion H0; subst. inversion H. inversion H.
+    replace t1'0 with t1'. reflexivity. apply IHstep.
+    assumption.
+  Qed.
+
+Theorem neg_strong_progress : exists t,
+  ~ value t /\ ~ (exists t', t => t').
+Proof.
+  exists (P (C 0) tfalse).
+  split; intros H; inversion H.
+  inversion H0; subst.
+  inversion H4.
+  inversion H5.
+  Qed.
+
+End Combined.
+
+Inductive aval : aexp -> Prop :=
+  av_num : forall n, aval (ANum n).
+
+Reserved Notation " t '/' st '==>a' t' " (at level 40, st at level 39).
+
+Inductive astep : state -> aexp -> aexp -> Prop :=
+  | AS_Id : forall st i, 
+      AId i / st ==>a ANum (st i)
+  | AS_Plus : forall st n1 n2,
+      APlus (ANum n1) (ANum n2) / st ==>a ANum (n1 + n2)
+  | AS_Plus1 : forall st a1 a1' a2,
+      a1 / st ==>a a1' ->
+      (APlus a1 a2) / st ==>a (APlus a1' a2)
+  | AS_Plus2 : forall st v1 a2 a2',
+      aval v1 ->
+      a2 / st ==>a a2' ->
+      (APlus v1 a2) / st ==>a (APlus v1 a2')
+  | AS_Minus : forall st n1 n2,
+      (AMinus (ANum n1) (ANum n2)) / st ==>a (ANum (minus n1 n2))
+  | AS_Minus1 : forall st a1 a1' a2,
+      a1 / st ==>a a1' ->
+      (AMinus a1 a2) / st ==>a (AMinus a1' a2)
+  | AS_Minus2 : forall st v1 a2 a2',
+      aval v1 ->
+      a2 / st ==>a a2' ->
+      (AMinus v1 a2) / st ==>a (AMinus v1 a2')
+  | AS_Mult : forall st n1 n2,
+      (AMult (ANum n1) (ANum n2)) / st ==>a (ANum (mult n1 n2))
+  | AS_Mult1 : forall st a1 a1' a2,
+      a1 / st ==>a a1' ->
+      (AMult (a1) (a2)) / st ==>a (AMult (a1') (a2))
+  | AS_Mult2 : forall st v1 a2 a2',
+      aval v1 ->
+      a2 / st ==>a a2' ->
+      (AMult v1 a2) / st ==>a (AMult v1 a2')
+
+    where " t '/' st '==>a' t' " := (astep st t t').
+
+Reserved Notation " t '/' st '==>b' t' " (at level 40, st at level 39).
+
+Inductive bstep : state -> bexp -> bexp -> Prop :=
+  | BS_Eq : forall st n1 n2,
+      (BEq (ANum n1) (ANum n2)) / st ==>b 
+      (if (beq_nat n1 n2) then BTrue else BFalse)
+  | BS_Eq1 : forall st a1 a1' a2,
+      a1 / st ==>a a1' ->
+      (BEq a1 a2) / st ==>b (BEq a1' a2)
+  | BS_Eq2 : forall st v1 a2 a2',
+      aval v1 -> 
+      a2 / st ==>a a2' ->
+      (BEq v1 a2) / st ==>b (BEq v1 a2')
+  | BS_LtEq : forall st n1 n2,
+      (BLe (ANum n1) (ANum n2)) / st ==>b 
+               (if (ble_nat n1 n2) then BTrue else BFalse)
+  | BS_LtEq1 : forall st a1 a1' a2,
+      a1 / st ==>a a1' ->
+      (BLe a1 a2) / st ==>b (BLe a1' a2)
+  | BS_LtEq2 : forall st v1 a2 a2',
+      aval v1 ->
+      a2 / st ==>a a2' ->
+      (BLe v1 a2) / st ==>b (BLe v1 (a2'))
+  | BS_NotTrue : forall st,
+      (BNot BTrue) / st ==>b BFalse
+  | BS_NotFalse : forall st,
+      (BNot BFalse) / st ==>b BTrue
+  | BS_NotStep : forall st b1 b1',
+      b1 / st ==>b b1' ->
+      (BNot b1) / st ==>b (BNot b1')
+  | BS_AndTrueTrue : forall st,
+      (BAnd BTrue BTrue) / st ==>b BTrue
+  | BS_AndTrueFalse : forall st,
+      (BAnd BTrue BFalse) / st ==>b BFalse
+  | BS_AndFalse : forall st b2,
+      (BAnd BFalse b2) / st ==>b BFalse
+  | BS_AndTrueStep : forall st b2 b2',
+      b2 / st ==>b b2' ->
+      (BAnd BTrue b2) / st ==>b (BAnd BTrue b2')
+  | BS_AndStep : forall st b1 b1' b2,
+      b1 / st ==>b b1' ->
+      (BAnd b1 b2) / st ==>b (BAnd b1' b2)
+
+  where " t '/' st '==>b' t' " := (bstep st t t').
+
+Reserved Notation " t '/' st '==>' t' '/' st' " 
+                  (at level 40, st at level 39, t' at level 39).
+
+Inductive cstep : (com * state) -> (com * state) -> Prop :=
+  | CS_AssStep : forall st i a a',
+      a / st ==>a a' ->
+      (i ::= a) / st ==> (i ::= a') / st 
+  | CS_Ass : forall st i n, 
+      (i ::= (ANum n)) / st ==> SKIP / (update st i n)
+  | CS_SeqStep : forall st c1 c1' st' c2,
+      c1 / st ==> c1' / st' ->
+      (c1 ;; c2) / st ==> (c1' ;; c2) / st'
+  | CS_SeqFinish : forall st c2,
+      (SKIP ;; c2) / st ==> c2 / st
+  | CS_IfTrue : forall st c1 c2,
+      IFB BTrue THEN c1 ELSE c2 FI / st ==> c1 / st
+  | CS_IfFalse : forall st c1 c2,
+      IFB BFalse THEN c1 ELSE c2 FI / st ==> c2 / st
+  | CS_IfStep : forall st b b' c1 c2,
+      b / st ==>b b' ->
+      IFB b THEN c1 ELSE c2 FI / st ==> (IFB b' THEN c1 ELSE c2 FI) / st
+  | CS_While : forall st b c1,
+          (WHILE b DO c1 END) / st
+      ==> (IFB b THEN (c1;; (WHILE b DO c1 END)) ELSE SKIP FI) / st
+
+  where " t '/' st '==>' t' '/' st' " := (cstep (t,st) (t',st')).
+
+Module CImp.
+
+Inductive com : Type :=
+  | CSkip : com
+  | CAss : id -> aexp -> com
+  | CSeq : com -> com -> com
+  | CIf : bexp -> com -> com -> com
+  | CWhile : bexp -> com -> com
+  | CPar : com -> com -> com.
+
+Tactic Notation "com_cases" tactic(first) ident(c) :=
+  first;
+  [ Case_aux c "SKIP" | Case_aux c "::=" | Case_aux c ";"
+  | Case_aux c "IFB" | Case_aux c "WHILE" | Case_aux c "PAR" ].
+
+Notation "'SKIP'" := 
+  CSkip.
+Notation "x '::=' a" := 
+  (CAss x a) (at level 60).
+Notation "c1 ;; c2" := 
+  (CSeq c1 c2) (at level 80, right associativity).
+Notation "'WHILE' b 'DO' c 'END'" := 
+  (CWhile b c) (at level 80, right associativity).
+Notation "'IFB' b 'THEN' c1 'ELSE' c2 'FI'" := 
+  (CIf b c1 c2) (at level 80, right associativity).
+Notation "'PAR' c1 'WITH' c2 'END'" := 
+  (CPar c1 c2) (at level 80, right associativity).
+
+Inductive cstep : (com * state)  -> (com * state) -> Prop :=
+  | CS_AssStep : forall st i a a',
+      a / st ==>a a' -> 
+      (i ::= a) / st ==> (i ::= a') / st
+  | CS_Ass : forall st i n, 
+      (i ::= (ANum n)) / st ==> SKIP / (update st i n)
+  | CS_SeqStep : forall st c1 c1' st' c2,
+      c1 / st ==> c1' / st' ->
+      (c1 ;; c2) / st ==> (c1' ;; c2) / st'
+  | CS_SeqFinish : forall st c2,
+      (SKIP ;; c2) / st ==> c2 / st
+  | CS_IfTrue : forall st c1 c2,
+      (IFB BTrue THEN c1 ELSE c2 FI) / st ==> c1 / st
+  | CS_IfFalse : forall st c1 c2,
+      (IFB BFalse THEN c1 ELSE c2 FI) / st ==> c2 / st
+  | CS_IfStep : forall st b b' c1 c2,
+      b /st ==>b b' -> 
+      (IFB b THEN c1 ELSE c2 FI) / st ==> (IFB b' THEN c1 ELSE c2 FI) / st
+  | CS_While : forall st b c1,
+      (WHILE b DO c1 END) / st ==> 
+               (IFB b THEN (c1;; (WHILE b DO c1 END)) ELSE SKIP FI) / st
+  | CS_Par1 : forall st c1 c1' c2 st',
+      c1 / st ==> c1' / st' -> 
+      (PAR c1 WITH c2 END) / st ==> (PAR c1' WITH c2 END) / st'
+  | CS_Par2 : forall st c1 c2 c2' st',
+      c2 / st ==> c2' / st' ->
+      (PAR c1 WITH c2 END) / st ==> (PAR c1 WITH c2' END) / st'
+  | CS_ParDone : forall st,
+      (PAR SKIP WITH SKIP END) / st ==> SKIP / st
+  where " t '/' st '==>' t' '/' st' " := (cstep (t,st) (t',st')).
+
+Definition cmultistep := multi cstep. 
+
+Notation " t '/' st '==>*' t' '/' st' " := 
+   (multi cstep  (t,st) (t',st')) 
+   (at level 40, st at level 39, t' at level 39).  
+
+Definition par_loop : com :=
+  PAR
+    Y ::= ANum 1
+  WITH
+    WHILE BEq (AId Y) (ANum 0) DO
+      X ::= APlus (AId X) (ANum 1)
+    END
+  END.
+
+Example par_loop_example_0:
+  exists st',
+       par_loop / empty_state  ==>* SKIP / st'
+    /\ st' X = 0.
+Proof.
+  eapply ex_intro. split.
+  unfold par_loop.
+  eapply multi_step. apply CS_Par1.
+    apply CS_Ass.
+  eapply multi_step. apply CS_Par2. apply CS_While.
+  eapply multi_step. apply CS_Par2. apply CS_IfStep. 
+    apply BS_Eq1. apply AS_Id.
+  eapply multi_step. apply CS_Par2. apply CS_IfStep. 
+    apply BS_Eq. simpl. 
+  eapply multi_step. apply CS_Par2. apply CS_IfFalse. 
+  eapply multi_step. apply CS_ParDone. 
+  eapply multi_refl. 
+  reflexivity. Qed.
+
+Example par_loop_example_2:
+  exists st',
+       par_loop / empty_state ==>* SKIP / st'
+    /\ st' X = 2.
+Proof.
+  eapply ex_intro. split.
+  eapply multi_step. apply CS_Par2. apply CS_While.
+  eapply multi_step. apply CS_Par2. apply CS_IfStep. 
+    apply BS_Eq1. apply AS_Id.
+  eapply multi_step. apply CS_Par2. apply CS_IfStep. 
+    apply BS_Eq. simpl. 
+  eapply multi_step. apply CS_Par2. apply CS_IfTrue. 
+  eapply multi_step. apply CS_Par2. apply CS_SeqStep.
+    apply CS_AssStep. apply AS_Plus1. apply AS_Id.
+  eapply multi_step. apply CS_Par2. apply CS_SeqStep.
+    apply CS_AssStep. apply AS_Plus.  
+  eapply multi_step. apply CS_Par2. apply CS_SeqStep.
+    apply CS_Ass.
+  eapply multi_step. apply CS_Par2. apply CS_SeqFinish.
+
+  eapply multi_step. apply CS_Par2. apply CS_While.
+  eapply multi_step. apply CS_Par2. apply CS_IfStep. 
+    apply BS_Eq1. apply AS_Id.
+  eapply multi_step. apply CS_Par2. apply CS_IfStep. 
+    apply BS_Eq. simpl. 
+  eapply multi_step. apply CS_Par2. apply CS_IfTrue. 
+  eapply multi_step. apply CS_Par2. apply CS_SeqStep.
+    apply CS_AssStep. apply AS_Plus1. apply AS_Id.
+  eapply multi_step. apply CS_Par2. apply CS_SeqStep.
+    apply CS_AssStep. apply AS_Plus.  
+  eapply multi_step. apply CS_Par2. apply CS_SeqStep.
+    apply CS_Ass.
+
+  eapply multi_step. apply CS_Par1. apply CS_Ass.
+  eapply multi_step. apply CS_Par2. apply CS_SeqFinish.
+  eapply multi_step. apply CS_Par2. apply CS_While.
+  eapply multi_step. apply CS_Par2. apply CS_IfStep. 
+    apply BS_Eq1. apply AS_Id.
+  eapply multi_step. apply CS_Par2. apply CS_IfStep. 
+    apply BS_Eq. simpl. 
+  eapply multi_step. apply CS_Par2. apply CS_IfFalse. 
+  eapply multi_step. apply CS_ParDone. 
+  eapply multi_refl. 
+  reflexivity. Qed. 
+
+Lemma par_body_n__Sn : forall n st,
+  st X = n /\ st Y = 0 ->
+  par_loop / st ==>* par_loop / (update st X (S n)).
+Proof.
+  intros. inversion H as [H1 H2]. subst.
+  eapply multi_step. apply CS_Par2. apply CS_While.
+  eapply multi_step. apply CS_Par2. apply CS_IfStep. 
+    apply BS_Eq1. apply AS_Id.
+  eapply multi_step. apply CS_Par2. apply CS_IfStep.
+    apply BS_Eq. rewrite H2. simpl.
+  eapply multi_step. apply CS_Par2. apply CS_IfTrue.
+  eapply multi_step. apply CS_Par2. apply CS_SeqStep.
+    apply CS_AssStep. apply AS_Plus1. apply AS_Id.
+  eapply multi_step. apply CS_Par2. apply CS_SeqStep.
+    apply CS_AssStep. apply AS_Plus.
+  eapply multi_step. apply CS_Par2. apply CS_SeqStep.
+    apply CS_Ass.
+  eapply multi_step. apply CS_Par2. apply CS_SeqFinish.
+  rewrite plus_comm. simpl.
+  apply multi_refl.
+  Qed.
+
+Lemma par_body_n : forall n st,
+  st X = 0 /\ st Y = 0 ->
+  exists st',
+    par_loop / st ==>*  par_loop / st' /\ st' X = n /\ st' Y = 0.
+Proof.
+  induction n; intros.
+    exists st. split. apply multi_refl.
+      assumption.
+    assert(exists st' : state,
+        par_loop / st ==>* par_loop / st' /\ st' X = n /\ st' Y = 0).
+    apply IHn. assumption. inversion H0.
+    exists (update x X (S n)).
+    split;
+    inversion H1 as [H2 H3]. 
+    eapply multi_trans. apply H2.
+    eapply par_body_n__Sn.
+    assumption. split.
+    rewrite update_eq. reflexivity.
+    inversion H3 as [H4 H5].
+    rewrite update_neq. assumption.
+    destruct (eq_id_dec X Y) eqn:xy; inversion xy.
+    assumption.
+  Qed.
+
+Theorem par_loop_any_X:
+  forall n, exists st',
+    par_loop / empty_state ==>*  SKIP / st'
+    /\ st' X = n.
+Proof.
+  intros n. 
+  destruct (par_body_n n empty_state). 
+    split; unfold update; reflexivity.
+
+  rename x into st.
+  inversion H as [H' [HX HY]]; clear H. 
+  exists (update st Y 1). split.
+  eapply multi_trans with (par_loop,st). apply H'. 
+  eapply multi_step. apply CS_Par1. apply CS_Ass.
+  eapply multi_step. apply CS_Par2. apply CS_While.
+  eapply multi_step. apply CS_Par2. apply CS_IfStep.
+    apply BS_Eq1. apply AS_Id. rewrite update_eq.
+  eapply multi_step. apply CS_Par2. apply CS_IfStep.
+    apply BS_Eq. simpl.
+  eapply multi_step. apply CS_Par2. apply CS_IfFalse.
+  eapply multi_step. apply CS_ParDone.
+  apply multi_refl.
+
+  rewrite update_neq. assumption. intro X; inversion X. 
+Qed.
+
+End CImp.
+
+Definition stack := list nat.
+Definition prog  := list sinstr.
+
+Inductive stack_step : state -> prog * stack -> prog * stack -> Prop :=
+  | SS_Push : forall st stk n p',
+    stack_step st (SPush n :: p', stk)      (p', n :: stk)
+  | SS_Load : forall st stk i p',
+    stack_step st (SLoad i :: p', stk)      (p', st i :: stk)
+  | SS_Plus : forall st stk n m p',
+    stack_step st (SPlus :: p', n::m::stk)  (p', (m+n)::stk)
+  | SS_Minus : forall st stk n m p',
+    stack_step st (SMinus :: p', n::m::stk) (p', (m-n)::stk)
+  | SS_Mult : forall st stk n m p',
+    stack_step st (SMult :: p', n::m::stk)  (p', (m*n)::stk).
+
+Theorem stack_step_deterministic : forall st, 
+  deterministic (stack_step st).
+Proof.
+  unfold deterministic. intros st x y1 y2 H1 H2.
+  induction H1; inversion H2; reflexivity.
+Qed.
+
+Definition stack_multistep st := multi (stack_step st).
+
+Definition compiler_is_correct_statement : Prop := forall e st stck,
+  stack_multistep st (s_compile e , stck) ([],(aeval st e)::stck).
+
+Theorem compiler_app : forall st e1 e2 stck stck' stck'',
+  stack_multistep st (e1 , stck) ([], stck') ->
+  stack_multistep st (e2 , stck') ([], stck'') ->
+  stack_multistep st (e1 ++ e2 , stck) ([],stck'').
+Proof.
+  intros st. induction e1; intros.
+    inversion H; subst. simpl. assumption.
+    inversion H1.
+  inversion H; subst.
+  inversion H1; subst; simpl;
+  eapply multi_step; try constructor; eapply IHe1; try apply H2; apply H0.
+  Qed.
+
+Theorem compiler_is_correct : compiler_is_correct_statement.
+Proof.
+  unfold compiler_is_correct_statement.
+  induction e; intros; simpl. 
+  eapply multi_step; try constructor.
+  eapply multi_step; try constructor.
+  eapply multi_trans; try eapply compiler_app; try apply IHe1;
+    try eapply compiler_app; try apply IHe2; econstructor; constructor.
+  eapply multi_trans; try eapply compiler_app; try apply IHe1;
+    try eapply compiler_app; try apply IHe2; econstructor; constructor.
+  eapply multi_trans; try eapply compiler_app; try apply IHe1;
+    try eapply compiler_app; try apply IHe2; econstructor; constructor.
+  Qed.
